Use normal function arrow → for `saved_pred_own`.

theories/base_logic/lib/saved_prop.v
@@ -90,19 +90,20 @@ Qed.
 Notation savedPredG Σ A := (savedAnythingG Σ (A -c> ▶ ∙)).
 Notation savedPredΣ A := (savedAnythingΣ (A -c> ▶ ∙)).
 
-Definition saved_pred_own `{savedPredG Σ A} (γ : gname) (Φ : A -c> iProp Σ) :=
+Definition saved_pred_own `{savedPredG Σ A} (γ : gname) (Φ : A → iProp Σ) :=
   saved_anything_own (F := A -c> ▶ ∙) γ (CofeMor Next ∘ Φ).
 
-Instance saved_pred_own_contractive `{savedPredG Σ A} γ : Contractive (saved_pred_own γ).
+Instance saved_pred_own_contractive `{savedPredG Σ A} γ :
+  Contractive (saved_pred_own γ : (A -c> iProp Σ) → iProp Σ).
 Proof.
   solve_proper_core ltac:(fun _ => first [ intros ?; progress simpl | by auto | f_contractive | f_equiv ]).
 Qed.
 
-Lemma saved_pred_alloc_strong `{savedPredG Σ A} (G : gset gname) (Φ : A -c> iProp Σ) :
+Lemma saved_pred_alloc_strong `{savedPredG Σ A} (G : gset gname) (Φ : A → iProp Σ) :
   (|==> ∃ γ, ⌜γ ∉ G⌝ ∧ saved_pred_own γ Φ)%I.
 Proof. iApply saved_anything_alloc_strong. Qed.
 
-Lemma saved_pred_alloc `{savedPredG Σ A} (Φ : A -c> iProp Σ) :
+Lemma saved_pred_alloc `{savedPredG Σ A} (Φ : A → iProp Σ) :
   (|==> ∃ γ, saved_pred_own γ Φ)%I.
 Proof. iApply saved_anything_alloc. Qed.
 
